\text{КДНФ:} $ f = \
\nx{1}\nx{2}\nx{3}\nx{4}\nx{5} \vee \
\nx{1}\nx{2}\x {3}\nx{4}\x {5} \vee \
\nx{1}\nx{2}\x {3}\x {4}\nx{5} \vee \
\nx{1}\nx{2}\x {3}\x {4}\x {5} \vee \
\nx{1}\x {2}\x {3}\nx{4}\x {5} \vee \
\nx{1}\x {2}\x {3}\x {4}\nx{5} \vee \
\nx{1}\x {2}\x {3}\x {4}\x {5} \vee \
\x {1}\nx{2}\nx{3}\x {4}\x {5} \vee \
\x {1}\nx{2}\x {3}\nx{4}\x {5} \vee \
\x {1}\nx{2}\x {3}\x {4}\nx{5} \vee \
\x {1}\x {2}\nx{3}\x {4}\nx{5} \vee \
\x {1}\x {2}\nx{3}\x {4}\x {5} \vee \
\x {1}\x {2}\x {3}\nx{4}\x {5}  \
$

ККНФ: $ f = \
(\x {1} \vee \x {2} \vee \x {3} \vee \x {4} \vee \nx{5})
(\x {1} \vee \x {2} \vee \x {3} \vee \nx{4} \vee \x {5})
(\x {1} \vee \x {2} \vee \x {3} \vee \nx{4} \vee \nx{5})
(\x {1} \vee \nx{2} \vee \x {3} \vee \x {4} \vee \x {5})
(\x {1} \vee \nx{2} \vee \x {3} \vee \x {4} \vee \nx{5})
(\x {1} \vee \nx{2} \vee \x {3} \vee \nx{4} \vee \x {5})
(\x {1} \vee \nx{2} \vee \x {3} \vee \nx{4} \vee \nx{5})
(\nx{1} \vee \x {2} \vee \x {3} \vee \x {4} \vee \x {5})
(\nx{1} \vee \x {2} \vee \x {3} \vee \x {4} \vee \nx{5})
(\nx{1} \vee \x {2} \vee \x {3} \vee \nx{4} \vee \x {5})
(\nx{1} \vee \x {2} \vee \nx{3} \vee \nx{4} \vee \nx{5})
(\nx{1} \vee \nx{2} \vee \x {3} \vee \x {4} \vee \x {5})
(\nx{1} \vee \nx{2} \vee \x {3} \vee \x {4} \vee \nx{5})
(\nx{1} \vee \nx{2} \vee \nx{3} \vee \nx{4} \vee \x {5})
(\nx{1} \vee \nx{2} \vee \nx{3} \vee \nx{4} \vee \nx{5})
$ \\\\

